#proof 
# to proove:
![[theorem composition of bijective function raw]]
## [[injectivity]]:
From $$g(f(x)) = g(f(y))$$ with $x,y\in X$. Because [[Function]] $g$ is [[injectivity|injective]] $$f(x)=f(y)$$ beacause of [[injectivity]] of $f$ follows $x=y$ 

## [[surjectivity]]:
for every [[element]] $z\in Z$, there is a $y\in Y$ with $g(y)=z$ because of [[surjectivity]] of $g$. for which in turn there exists an $x\in X$ with $f(x) = y$. this means that every for every $z\in Z$ there exists a [[preimage]] $x\in X$ regarding $g\circ f$. $\begin{equation}\begin{aligned}x&=4\\&=7\end{aligned}\end{equation}$ 

