# **theorem of the [[inverse function]]**
if $f:X\to Y$ is a [[bijectivity|bijective]] [[Function]], there exists a [[Function]] $g:Y\to X$ with: 
	$g\circ f = id_X \text{ and } f\circ g = id_Y$
more precicely:

**there exists an [[inverse function]] if and only if the [[Function]] is [[bijectivity|bijective]]** 

we call this [[Function]] the [[inverse function]] of $f$, which is denounced as $f^{-1}$. The
[[Function]] $f^{-1}$ is also [[bijectivity|bijective]] and has the [[inverse function]] $(f^{-1})^{-1}=f$ 
#theorem 